# Prompt #46: Point P = (1, 2, −4). Rotate P 120° around the axis through the origin in direction ⟨1, 1, 1⟩ (right-hand rule). Give the exact coordinates.

## OpenAI o3  (27 secs)
Let  

v = (1, 2, −4) (the position-vector of P)  
k = (1, 1, 1) / √3 (unit vector along the axis)  
θ = 120° = 2π/3.

Use Rodrigues’ rotation formula  
v′ = v cos θ + (k × v) sin θ + k(k·v)(1 – cos θ).

Step 1.  k·v  
k·v = (1+2−4)/√3 = −1/√3.

Step 2.  k × v  
(1,1,1) × (1,2,−4) = (−6, 5, 1)  
⇒ k × v = (−6, 5, 1)/√3.

Step 3.  Trigonometric factors  
cos θ = −1/2, sin θ = √3/2, 1 – cos θ = 3/2.

Step 4.  Assemble the terms  
v cos θ = (1,2,−4)(−1/2) = (−1/2, −1, 2)  

(k × v) sin θ = (−6, 5, 1)/√3 · √3/2 = (−3, 5/2, 1/2)  

k(k·v)(1 – cos θ) = (1,1,1)/√3 · (−1/√3) · 3/2 = (−1/2, −1/2, −1/2).

Add them:  
(−1/2, −1, 2) + (−3, 5/2, 1/2) + (−1/2, −1/2, −1/2) = (−4, 1, 2).

Therefore the exact coordinates of the rotated point are  

P′ = (−4, 1, 2).

## Claude 4 Sonnet  (24 secs)
I need to find the coordinates of point P after rotating it 120° around the axis through the origin in direction ⟨1, 1, 1⟩.

First, let me normalize the axis vector:
- v = ⟨1, 1, 1⟩
- |v| = √(1² + 1² + 1²) = √3
- Unit vector: u = ⟨1/√3, 1/√3, 1/√3⟩

For rotation by angle θ around a unit vector u = ⟨u₁, u₂, u₃⟩, I'll use Rodrigues' rotation formula:
**R(P) = P cos θ + (u × P) sin θ + u(u · P)(1 - cos θ)**

Given values:
- P = ⟨1, 2, -4⟩
- θ = 120° = 2π/3
- cos(120°) = -1/2
- sin(120°) = √3/2
- u = ⟨1/√3, 1/√3, 1/√3⟩

Let me calculate each component:

**1) u · P** (dot product):
u · P = (1/√3)(1) + (1/√3)(2) + (1/√3)(-4) = (1 + 2 - 4)/√3 = -1/√3

**2) u × P** (cross product):
u × P = |i  j  k|
        |1/√3  1/√3  1/√3|
        |1  2  -4|

= i[(1/√3)(-4) - (1/√3)(2)] - j[(1/√3)(-4) - (1/√3)(1)] + k[(1/√3)(2) - (1/√3)(1)]
= i[-6/√3] - j[-5/√3] + k[1/√3]
= ⟨-6/√3, 5/√3, 1/√3⟩

**3) Now applying Rodrigues' formula:**

R(P) = P cos θ + (u × P) sin θ + u(u · P)(1 - cos θ)

= ⟨1, 2, -4⟩(-1/2) + ⟨-6/√3, 5/√3, 1/√3⟩(√3/2) + ⟨1/√3, 1/√3, 1/√3⟩(-1/√3)(3/2)

= ⟨-1/2, -1, 2⟩ + ⟨-6/√3 · √3/2, 5/√3 · √3/2, 1/√3 · √3/2⟩ + ⟨1/√3, 1/√3, 1/√3⟩(-3/2√3)

= ⟨-1/2, -1, 2⟩ + ⟨-3, 5/2, 1/2⟩ + ⟨-1/2, -1/2, -1/2⟩

= ⟨-1/2 - 3 - 1/2, -1 + 5/2 - 1/2, 2 + 1/2 - 1/2⟩

= ⟨-4, 1, 2⟩

Therefore, the exact coordinates after rotation are **(-4, 1, 2)**.

## Gemini Pro  (106 secs)
Let P = ⟨1, 2, -4⟩ be the vector representing the point P from the origin.
Let the axis of rotation be defined by the unit vector u. The direction vector is v = ⟨1, 1, 1⟩.
The norm of v is ||v|| = √(1² + 1² + 1²) = √3.
So, the unit vector u is u = (1/√3)⟨1, 1, 1⟩.
The angle of rotation is θ = 120°.
We use Rodrigues' rotation formula to find the rotated vector P':
P' = P cos θ + (u × P) sin θ + u (u · P) (1 - cos θ).

First, let's calculate the values of cos θ and sin θ:
cos θ = cos(120°) = -1/2.
sin θ = sin(120°) = √3/2.
Also, 1 - cos θ = 1 - (-1/2) = 3/2.

Next, we calculate the dot product u · P:
u · P = (1/√3)(1) * 1 + (1/√3)(1) * 2 + (1/√3)(1) * (-4)
= (1/√3)(1 + 2 - 4) = (1/√3)(-1) = -1/√3.

Next, we calculate the cross product u × P:
u × P = (1/√3)⟨1, 1, 1⟩ × ⟨1, 2, -4⟩.
The cross product ⟨1, 1, 1⟩ × ⟨1, 2, -4⟩ is:
i((1)(-4) - (1)(2)) - j((1)(-4) - (1)(1)) + k((1)(2) - (1)(1))
= i(-4 - 2) - j(-4 - 1) + k(2 - 1)
= -6i + 5j + 1k = ⟨-6, 5, 1⟩.
So, u × P = (1/√3)⟨-6, 5, 1⟩.

Now we can substitute these values into Rodrigues' formula. It consists of three terms:
1. P cos θ = ⟨1, 2, -4⟩ * (-1/2) = ⟨-1/2, -1, 2⟩.
2. (u × P) sin θ = (1/√3)⟨-6, 5, 1⟩ * (√3/2) = (1/2)⟨-6, 5, 1⟩ = ⟨-3, 5/2, 1/2⟩.
3. u (u · P) (1 - cos θ) = ⟨1/√3, 1/√3, 1/√3⟩ * (-1/√3) * (3/2).
   This simplifies to (1/3)⟨1, 1, 1⟩ * (-1) * (3/2) = (-1/2)⟨1, 1, 1⟩ = ⟨-1/2, -1/2, -1/2⟩.

Finally, sum these three terms to get P':
P' = ⟨-1/2, -1, 2⟩ + ⟨-3, 5/2, 1/2⟩ + ⟨-1/2, -1/2, -1/2⟩.
P'_x = -1/2 - 3 - 1/2 = -1 - 3 = -4.
P'_y = -1 + 5/2 - 1/2 = -1 + (5/2 - 1/2) = -1 + 4/2 = -1 + 2 = 1.
P'_z = 2 + 1/2 - 1/2 = 2.

So the coordinates of the rotated point P' are ⟨-4, 1, 2⟩.

Alternative method using rotation matrix:
The rotation matrix for a rotation by angle θ around an axis u = (u_x, u_y, u_z) is given by R =
cosθ I + sinθ [u]_× + (1-cosθ) u u^T
where I is the identity matrix, [u]_× is the cross-product matrix of u:
[u]_× = [[0, -u_z, u_y], [u_z, 0, -u_x], [-u_y, u_x, 0]]
and u u^T is the outer product of u with itself.
u = ⟨1/√3, 1/√3, 1/√3⟩. So u_x=u_y=u_z=1/√3.
cosθ = -1/2, sinθ = √3/2, 1-cosθ = 3/2.

cosθ I = [[-1/2, 0, 0], [0, -1/2, 0], [0, 0, -1/2]].

sinθ [u]_× = (√3/2) * (1/√3) * [[0, -1, 1], [1, 0, -1], [-1, 1, 0]]
= (1/2) * [[0, -1, 1], [1, 0, -1], [-1, 1, 0]] = [[0, -1/2, 1/2], [1/2, 0, -1/2], [-1/2, 1/2, 0]].

(1-cosθ) u u^T = (3/2) * (1/√3)^2 * [[1,1,1],[1,1,1],[1,1,1]]
= (3/2) * (1/3) * [[1,1,1],[1,1,1],[1,1,1]] = (1/2) * [[1,1,1],[1,1,1],[1,1,1]]
= [[1/2, 1/2, 1/2], [1/2, 1/2, 1/2], [1/2, 1/2, 1/2]].

Summing these matrices:
R = [[-1/2+0+1/2, 0-1/2+1/2, 0+1/2+1/2],
     [0+1/2+1/2, -1/2+0+1/2, 0-1/2+1/2],
     [0-1/2+1/2, 0+1/2+1/2, -1/2+0+1/2]]
R = [[0, 0, 1], [1, 0, 0], [0, 1, 0]].

Now, apply this rotation matrix to P = ⟨1, 2, -4⟩:
P' = R P = [[0,0,1],[1,0,0],[0,1,0]] * [[1],[2],[-4]]
P'_x = (0)(1) + (0)(2) + (1)(-4) = -4.
P'_y = (1)(1) + (0)(2) + (0)(-4) = 1.
P'_z = (0)(1) + (1)(2) + (0)(-4) = 2.
So P' = ⟨-4, 1, 2⟩.
This matrix implies that if P=(x,y,z), then P'=(z,x,y). For P=(1,2,-4), P'=(-4,1,2). This is a known property for 120° rotation around the ⟨1,1,1⟩ axis.

The coordinates of the rotated point are (-4, 1, 2).

The final answer is $\boxed{(-4, 1, 2)}$.

## DeepSeek Reasoner  (437 secs)
To rotate point \(P = (1, 2, -4)\) by 120° around the axis through the origin in the direction \(\langle 1, 1, 1 \rangle\) using the right-hand rule, Rodrigues' rotation formula is applied. The formula for rotating a vector \(\mathbf{v}\) by an angle \(\theta\) around a unit vector \(\mathbf{u}\) is:

\[
\mathbf{v}' = \mathbf{v} \cos \theta + (\mathbf{u} \times \mathbf{v}) \sin \theta + \mathbf{u} (\mathbf{u} \cdot \mathbf{v}) (1 - \cos \theta)
\]

The axis vector is \(\mathbf{a} = \langle 1, 1, 1 \rangle\), with magnitude \(\|\mathbf{a}\| = \sqrt{1^2 + 1^2 + 1^2} = \sqrt{3}\). The unit vector \(\mathbf{u}\) is:

\[
\mathbf{u} = \frac{\mathbf{a}}{\|\mathbf{a}\|} = \left\langle \frac{1}{\sqrt{3}}, \frac{1}{\sqrt{3}}, \frac{1}{\sqrt{3}}} \right\rangle
\]

The vector to rotate is \(\mathbf{v} = \langle 1, 2, -4 \rangle\). The angle \(\theta = 120^\circ\), so:

\[
\cos 120^\circ = -\frac{1}{2}, \quad \sin 120^\circ = \frac{\sqrt{3}}{2}
\]

First, compute the dot product \(\mathbf{u} \cdot \mathbf{v}\):

\[
\mathbf{u} \cdot \mathbf{v} = \left( \frac{1}{\sqrt{3}} \right)(1) + \left( \frac{1}{\sqrt{3}} \right)(2) + \left( \frac{1}{\sqrt{3}} \right)(-4) = \frac{1}{\sqrt{3}} (1 + 2 - 4) = \frac{-1}{\sqrt{3}}
\]

Next, compute the cross product \(\mathbf{u} \times \mathbf{v}\):

\[
\mathbf{u} \times \mathbf{v} = \begin{vmatrix}
\mathbf{i} & \mathbf{j} & \mathbf{k} \\
\frac{1}{\sqrt{3}} & \frac{1}{\sqrt{3}} & \frac{1}{\sqrt{3}} \\
1 & 2 & -4 \\
\end{vmatrix} = \mathbf{i} \left( \frac{1}{\sqrt{3}} \cdot (-4) - \frac{1}{\sqrt{3}} \cdot 2 \right) - \mathbf{j} \left( \frac{1}{\sqrt{3}} \cdot (-4) - \frac{1}{\sqrt{3}} \cdot 1 \right) + \mathbf{k} \left( \frac{1}{\sqrt{3}} \cdot 2 - \frac{1}{\sqrt{3}} \cdot 1 \right)
\]

\[
= \mathbf{i} \left( -\frac{4}{\sqrt{3}} - \frac{2}{\sqrt{3}} \right) - \mathbf{j} \left( -\frac{4}{\sqrt{3}} - \frac{1}{\sqrt{3}} \right) + \mathbf{k} \left( \frac{2}{\sqrt{3}} - \frac{1}{\sqrt{3}} \right) = \mathbf{i} \left( -\frac{6}{\sqrt{3}} \right) - \mathbf{j} \left( -\frac{5}{\sqrt{3}} \right) + \mathbf{k} \left( \frac{1}{\sqrt{3}} \right)
\]

\[
= \left\langle -\frac{6}{\sqrt{3}}, \frac{5}{\sqrt{3}}, \frac{1}{\sqrt{3}}} \right\rangle
\]

Now compute each term in Rodrigues' formula:

1. \(\mathbf{v} \cos \theta = \langle 1, 2, -4 \rangle \cdot \left( -\frac{1}{2} \right) = \left\langle -\frac{1}{2}, -1, 2 \right\rangle\)

2. \((\mathbf{u} \times \mathbf{v}) \sin \theta = \left\langle -\frac{6}{\sqrt{3}}, \frac{5}{\sqrt{3}}, \frac{1}{\sqrt{3}}} \right\rangle \cdot \frac{\sqrt{3}}{2} = \left\langle -\frac{6}{\sqrt{3}} \cdot \frac{\sqrt{3}}{2}, \frac{5}{\sqrt{3}} \cdot \frac{\sqrt{3}}{2}, \frac{1}{\sqrt{3}} \cdot \frac{\sqrt{3}}{2} \right\rangle = \left\langle -3, \frac{5}{2}, \frac{1}{2} \right\rangle\)

3. \(\mathbf{u} (\mathbf{u} \cdot \mathbf{v}) (1 - \cos \theta) = \left\langle \frac{1}{\sqrt{3}}, \frac{1}{\sqrt{3}}, \frac{1}{\sqrt{3}}} \right\rangle \cdot \left( \frac{-1}{\sqrt{3}} \right) \cdot \left( 1 - \left( -\frac{1}{2} \right) \right) = \left\langle \frac{1}{\sqrt{3}}, \frac{1}{\sqrt{3}}, \frac{1}{\sqrt{3}}} \right\rangle \cdot \left( \frac{-1}{\sqrt{3}} \right) \cdot \frac{3}{2}\)

\[
= \left\langle \frac{1}{\sqrt{3}}, \frac{1}{\sqrt{3}}, \frac{1}{\sqrt{3}}} \right\rangle \cdot \left( -\frac{3}{2\sqrt{3}} \right) = \left\langle \frac{1}{\sqrt{3}} \cdot \left( -\frac{3}{2\sqrt{3}} \right), \frac{1}{\sqrt{3}} \cdot \left( -\frac{3}{2\sqrt{3}} \right), \frac{1}{\sqrt{3}} \cdot \left( -\frac{3}{2\sqrt{3}} \right) \right\rangle = \left\langle -\frac{1}{2}, -\frac{1}{2}, -\frac{1}{2} \right\rangle
\]

Sum the components:

- \(x\)-component: \(-\frac{1}{2} + (-3) + \left( -\frac{1}{2} \right) = -4\)
- \(y\)-component: \(-1 + \frac{5}{2} + \left( -\frac{1}{2} \right) = -1 + 2 = 1\)
- \(z\)-component: \(2 + \frac{1}{2} + \left( -\frac{1}{2} \right) = 2\)

Thus, the rotated vector is \(\langle -4, 1, 2 \rangle\).

The rotation can also be represented by the matrix that maps \((x, y, z)\) to \((z, x, y)\), confirming the result:

\[
\begin{pmatrix} 0 & 0 & 1 \\ 1 & 0 & 0 \\ 0 & 1 & 0 \end{pmatrix} \begin{pmatrix} 1 \\ 2 \\ -4 \end{pmatrix} = \begin{pmatrix} -4 \\ 1 \\ 2 \end{pmatrix}
\]

The dot product with the axis vector and the magnitude are preserved, and the rotation direction is consistent with the right-hand rule. The exact coordinates of the rotated point are \((-4, 1, 2)\).

\boxed{(-4,\ 1,\ 2)}

## Grok 3  (16 secs)
To rotate a point \( P = (1, 2, -4) \) by 120° around an axis through the origin in the direction of the vector \( \langle 1, 1, 1 \rangle \) using the right-hand rule, we will use the rotation matrix derived from the axis-angle representation. Let's proceed step by step.

---

### Step 1: Normalize the axis vector
The axis of rotation is given by the vector \( \mathbf{u} = \langle 1, 1, 1 \rangle \). First, we normalize it to get a unit vector.

The magnitude of \( \mathbf{u} \) is:
\[
|\mathbf{u}| = \sqrt{1^2 + 1^2 + 1^2} = \sqrt{3}
\]
Thus, the unit vector is:
\[
\hat{\mathbf{u}} = \left\langle \frac{1}{\sqrt{3}}, \frac{1}{\sqrt{3}}, \frac{1}{\sqrt{3}} \right\rangle
\]
Let \( u_x = u_y = u_z = \frac{1}{\sqrt{3}} \).

---

### Step 2: Set up the rotation matrix
The rotation matrix for a rotation by an angle \( \theta \) around an axis defined by a unit vector \( \hat{\mathbf{u}} = \langle u_x, u_y, u_z \rangle \) is given by:
\[
R = \begin{bmatrix}
\cos\theta + u_x^2(1 - \cos\theta) & u_x u_y (1 - \cos\theta) - u_z \sin\theta & u_x u_z (1 - \cos\theta) + u_y \sin\theta \\
u_y u_x (1 - \cos\theta) + u_z \sin\theta & \cos\theta + u_y^2(1 - \cos\theta) & u_y u_z (1 - \cos\theta) - u_x \sin\theta \\
u_z u_x (1 - \cos\theta) - u_y \sin\theta & u_z u_y (1 - \cos\theta) + u_x \sin\theta & \cos\theta + u_z^2(1 - \cos\theta)
\end{bmatrix}
\]
Here, \( \theta = 120^\circ \). Compute \( \cos\theta \) and \( \sin\theta \):
\[
\cos 120^\circ = -\frac{1}{2}, \quad \sin 120^\circ = \frac{\sqrt{3}}{2}
\]
Also, since \( u_x = u_y = u_z = \frac{1}{\sqrt{3}} \), we have:
\[
u_x^2 = u_y^2 = u_z^2 = \frac{1}{3}
\]
\[
u_x u_y = u_x u_z = u_y u_z = \frac{1}{3}
\]

Now compute the terms:
- \( 1 - \cos\theta = 1 - (-\frac{1}{2}) = \frac{3}{2} \)
- \( u_x^2 (1 - \cos\theta) = \frac{1}{3} \cdot \frac{3}{2} = \frac{1}{2} \)
- Similarly, \( u_y^2 (1 - \cos\theta) = u_z^2 (1 - \cos\theta) = \frac{1}{2} \)
- \( u_x u_y (1 - \cos\theta) = \frac{1}{3} \cdot \frac{3}{2} = \frac{1}{2} \), and same for other products
- \( u_z \sin\theta = \frac{1}{\sqrt{3}} \cdot \frac{\sqrt{3}}{2} = \frac{1}{2} \), and similarly for others

Now substitute into the matrix:
- Diagonal terms (e.g., first row, first column):
  \[
  \cos\theta + u_x^2 (1 - \cos\theta) = -\frac{1}{2} + \frac{1}{2} = 0
  \]
- Off-diagonal terms (e.g., first row, second column):
  \[
  u_x u_y (1 - \cos\theta) - u_z \sin\theta = \frac{1}{2} - \frac{1}{2} = 0
  \]
- First row, third column:
  \[
  u_x u_z (1 - \cos\theta) + u_y \sin\theta = \frac{1}{2} + \frac{1}{2} = 1
  \]

After computing all elements, the rotation matrix is:
\[
R = \begin{bmatrix}
0 & 0 & 1 \\
1 & 0 & 0 \\
0 & 1 & 0
\end{bmatrix}
\]

(Let me double-check the calculations to ensure correctness.)

Recompute key terms to avoid errors:
- \( \cos\theta = -\frac{1}{2} \)
- \( 1 - \cos\theta = \frac{3}{2} \)
- \( u_x^2 = \frac{1}{3} \), so \( u_x^2 (1 - \cos\theta) = \frac{1}{3} \cdot \frac{3}{2} = \frac{1}{2} \)
- Diagonal term: \( \cos\theta + u_x^2 (1 - \cos\theta) = -\frac{1}{2} + \frac{1}{2} = 0 \), correct
- Off-diagonal, e.g., \( u_x u_y (1 - \cos\theta) = \frac{1}{3} \cdot \frac{3}{2} = \frac{1}{2} \)
- \( u_z \sin\theta = \frac{1}{\sqrt{3}} \cdot \frac{\sqrt{3}}{2} = \frac{1}{2} \)
- So, \( u_x u_y (1 - \cos\theta) - u_z \sin\theta = \frac{1}{2} - \frac{1}{2} = 0 \), correct
- \( u_x u_z (1 - \cos\theta) + u_y \sin\theta = \frac{1}{2} + \frac{1}{2} = 1 \), correct

The matrix is indeed:
\[
R = \begin{bmatrix}
0 & 0 & 1 \\
1 & 0 & 0 \\
0 & 1 & 0
\end{bmatrix}
\]

---

### Step 3: Apply the rotation matrix to point P
The point \( P = (1, 2, -4) \) is represented as a column vector. The rotated point \( P' \) is given by:
\[
P' = R \cdot P
\]
\[
P' = \begin{bmatrix}
0 & 0 & 1 \\
1 & 0 & 0 \\
0 & 1 & 0
\end{bmatrix}
\begin{bmatrix}
1 \\
2 \\
-4
\end{bmatrix}
= \begin{bmatrix}
0 \cdot 1 + 0 \cdot 2 + 1 \cdot (-4) \\
1 \cdot 1 + 0 \cdot 2 + 0 \cdot (-4) \\
0 \cdot 1 + 1 \cdot 2 + 0 \cdot (-4)
\end{bmatrix}
= \begin{bmatrix}
-4 \\
1 \\
2
\end{bmatrix}
\]

---

### Step 4: Verify the result
The axis \( \langle 1, 1, 1 \rangle \) suggests a rotation that permutes the coordinates, and a 120° rotation around this axis (which is the body diagonal of a cube) should indeed cycle the coordinates. The matrix we obtained corresponds to a cyclic permutation \( (x, y, z) \to (z, x, y) \), which matches our computation: \( (1, 2, -4) \to (-4, 1, 2) \). This is consistent with a 120° rotation around the axis \( \langle 1, 1, 1 \rangle \).

---

### Final Answer
The exact coordinates of the rotated point are:
\[
\boxed{(-4, 1, 2)}
\]

