# Prompt #7: Gripper frame G is rotated 30° about X relative to robot frame R. Tool frame T is rotated 45° about Y relative to G. Give me the 3 × 3 rotation matrix from T to R.

## OpenAI o3

Let

• Rₓ(θ) be a right-hand rotation about the X–axis\
• Rᵧ(φ) be a right-hand rotation about the Y–axis

1. G relative to R: 30° about X\
   R_R^G = Rₓ(30°) = ⎡1  0  0 ⎤\
   ⎢0 cos30° −sin30°⎥\
   ⎣0 sin30° cos30°⎦

1. T relative to G: 45° about Y\
   R_G^T = Rᵧ(45°) = ⎡cos45° 0 sin45°⎤\
   ⎢ 0 1 0 ⎥\
   ⎣−sin45° 0 cos45°⎦

1. T relative to R (T → R):\
   R_R^T = R_R^G · R_G^T

Using cos30° = √3/2, sin30° = 1/2, cos45° = sin45° = √2/2,

R_R^T = ⎡ √2/2 0 √2/2 ⎤\
⎢ √2/4 √3/2 −√2/4 ⎥\
⎣−√6/4 1/2 √6/4 ⎦

Numerically (4-decimal rounding):

R_R^T ≈ ⎡ 0.7071 0 0.7071 ⎤\
⎢ 0.3536 0.8660 −0.3536⎥\
⎣−0.6124 0.5000 0.6124 ⎦

This 3 × 3 matrix converts a vector expressed in the tool frame T into the robot base frame R.

## Claude 4 Sonnet

I need to find the rotation matrix from tool frame T to robot frame R, which I'll denote as R_R^T.

Given information:

- Gripper frame G is rotated 30° about X relative to robot frame R
- Tool frame T is rotated 45° about Y relative to gripper frame G

First, let me establish the rotation matrices:

**Rotation from R to G (30° about X):**

```
R_G^R = Rx(30°) = [1    0         0    ]
                   [0  cos(30°) -sin(30°)]
                   [0  sin(30°)  cos(30°)]

R_G^R = [1    0       0   ]
        [0  √3/2    -1/2  ]
        [0   1/2     √3/2 ]
```

**Rotation from G to T (45° about Y):**

```
R_T^G = Ry(45°) = [cos(45°)   0   sin(45°)]
                   [   0       1      0    ]
                   [-sin(45°)  0   cos(45°)]

R_T^G = [√2/2    0    √2/2 ]
        [ 0      1     0   ]
        [-√2/2   0    √2/2 ]
```

**To find R_R^T (rotation from T to R):**

The rotation from T to R can be found by composing the rotations:
R_R^T = R_G^R × R_T^G

```
R_R^T = [1    0       0   ] × [√2/2    0    √2/2 ]
        [0  √3/2    -1/2  ]   [ 0      1     0   ]
        [0   1/2     √3/2 ]   [-√2/2   0    √2/2 ]
```

Performing the matrix multiplication:

Row 1: [√2/2, 0, √2/2]

Row 2: [√2/4, √3/2, √2/4]

Row 3: [-√6/4, 1/2, √6/4]

Therefore, the rotation matrix from T to R is:

```
R_R^T = [√2/2    0     √2/2 ]
        [√2/4   √3/2   √2/4 ]
        [-√6/4   1/2   √6/4 ]
```

Or in decimal form (approximately):

```
R_R^T = [ 0.707    0      0.707]
        [ 0.354   0.866   0.354]
        [-0.612   0.5     0.612]
```

## Gemini Pro

Okay, let's break this down.

We want to find the rotation matrix `R_R_T` (from Tool frame T to Robot frame R).
We are given:

1. Rotation from Robot frame (R) to Gripper frame (G): `R_R_G`. This is a rotation of 30° about the X-axis of R.
1. Rotation from Gripper frame (G) to Tool frame (T): `R_G_T`. This is a rotation of 45° about the Y-axis of G.

The relationship is:
`R_R_T = R_R_G * R_G_T`

**Step 1: Calculate `R_R_G` (Rotation of 30° about X_R)**
The basic rotation matrix about the X-axis is:

```
Rx(θ) = | 1    0        0      |
        | 0  cos(θ)  -sin(θ) |
        | 0  sin(θ)   cos(θ) |
```

For θ = 30°:
cos(30°) = √3/2
sin(30°) = 1/2

So,

```
R_R_G = | 1    0        0      |
        | 0  √3/2    -1/2    |
        | 0   1/2     √3/2   |
```

Numerically (approx):

```
R_R_G ≈ | 1    0        0      |
        | 0  0.866   -0.5    |
        | 0  0.5     0.866  |
```

**Step 2: Calculate `R_G_T` (Rotation of 45° about Y_G)**
The basic rotation matrix about the Y-axis is:

```
Ry(φ) = | cos(φ)   0   sin(φ) |
        |   0      1     0    |
        |-sin(φ)   0   cos(φ) |
```

For φ = 45°:
cos(45°) = √2/2
sin(45°) = √2/2

So,

```
R_G_T = | √2/2   0   √2/2 |
        |   0    1     0    |
        |-√2/2   0   √2/2 |
```

Numerically (approx):

```
R_G_T ≈ | 0.707   0   0.707 |
        |   0     1     0    |
        |-0.707   0   0.707 |
```

**Step 3: Calculate `R_R_T = R_R_G * R_G_T`**

```
R_R_T =   | 1    0        0      |   | √2/2   0   √2/2 |
          | 0  √3/2    -1/2    | * |   0    1     0    |
          | 0   1/2     √3/2   |   |-√2/2   0   √2/2 |
```

Performing the matrix multiplication:

- R_R_T(1,1) = (1 * √2/2) + (0 * 0) + (0 * -√2/2) = √2/2

- R_R_T(1,2) = (1 * 0) + (0 * 1) + (0 * 0) = 0

- R_R_T(1,3) = (1 * √2/2) + (0 * 0) + (0 * √2/2) = √2/2

- R_R_T(2,1) = (0 * √2/2) + (√3/2 * 0) + (-1/2 * -√2/2) = √2/4

- R_R_T(2,2) = (0 * 0) + (√3/2 * 1) + (-1/2 * 0) = √3/2

- R_R_T(2,3) = (0 * √2/2) + (√3/2 * 0) + (-1/2 * √2/2) = -√2/4

- R_R_T(3,1) = (0 * √2/2) + (1/2 * 0) + (√3/2 * -√2/2) = -√6/4

- R_R_T(3,2) = (0 * 0) + (1/2 * 1) + (√3/2 * 0) = 1/2

- R_R_T(3,3) = (0 * √2/2) + (1/2 * 0) + (√3/2 * √2/2) = √6/4

So, the final rotation matrix `R_R_T` is:

```
R_R_T = |  √2/2    0      √2/2   |
        |  √2/4   √3/2   -√2/4   |
        | -√6/4    1/2    √6/4   |
```

Numerically, this is approximately:

```
R_R_T ≈ |  0.7071    0       0.7071  |
        |  0.3536    0.8660 -0.3536  |
        | -0.6124    0.5     0.6124  |
```

## DeepSeek Reasoner

The rotation matrix from the tool frame T to the robot frame R is obtained by composing the rotations from T to the gripper frame G and from G to R.

First, the gripper frame G is rotated 30° about the X-axis relative to the robot frame R. The rotation matrix from G to R is the inverse of the rotation from R to G, which is a rotation about X by -30°. The rotation matrix for a rotation about X by an angle θ is:

```math
\[
R_x(\theta) = \begin{pmatrix}
1 & 0 & 0 \\
0 & \cos\theta & -\sin\theta \\
0 & \sin\theta & \cos\theta
\end{pmatrix}
\]

For θ = -30°:
- \(\cos(-30^\circ) = \cos(30^\circ) = \sqrt{3}/2\)
- \(\sin(-30^\circ) = -\sin(30^\circ) = -1/2\)

Thus:
\[
R_x(-30^\circ) = \begin{pmatrix}
1 & 0 & 0 \\
0 & \sqrt{3}/2 & 1/2 \\
0 & -1/2 & \sqrt{3}/2
\end{pmatrix}
\]

This is the rotation matrix from G to R, denoted as \(^R\mathbf{R}_G\).

Next, the tool frame T is rotated 45° about the Y-axis relative to the gripper frame G. The rotation matrix from T to G is the inverse of the rotation from G to T, which is a rotation about Y by -45°. The rotation matrix for a rotation about Y by an angle φ is:

\[
R_y(\phi) = \begin{pmatrix}
\cos\phi & 0 & \sin\phi \\
0 & 1 & 0 \\
-\sin\phi & 0 & \cos\phi
\end{pmatrix}
\]

For φ = -45°:
- \(\cos(-45^\circ) = \cos(45^\circ) = \sqrt{2}/2\)
- \(\sin(-45^\circ) = -\sin(45^\circ) = -\sqrt{2}/2\)

Thus:
\[
R_y(-45^\circ) = \begin{pmatrix}
\sqrt{2}/2 & 0 & -\sqrt{2}/2 \\
0 & 1 & 0 \\
\sqrt{2}/2 & 0 & \sqrt{2}/2
\end{pmatrix}
\]

This is the rotation matrix from T to G, denoted as \(^G\mathbf{R}_T\).

The rotation matrix from T to R is the product of the rotation from G to R and the rotation from T to G:
\[
^R\mathbf{R}_T = ^R\mathbf{R}_G \cdot ^G\mathbf{R}_T = R_x(-30^\circ) \cdot R_y(-45^\circ)
\]

Compute the product:
\[
R_x(-30^\circ) \cdot R_y(-45^\circ) = \begin{pmatrix}
1 & 0 & 0 \\
0 & \sqrt{3}/2 & 1/2 \\
0 & -1/2 & \sqrt{3}/2
\end{pmatrix} \cdot \begin{pmatrix}
\sqrt{2}/2 & 0 & -\sqrt{2}/2 \\
0 & 1 & 0 \\
\sqrt{2}/2 & 0 & \sqrt{2}/2
\end{pmatrix}
\]
```

Perform matrix multiplication:

```math
- **First row:**
  - First element: \(1 \cdot \sqrt{2}/2 + 0 \cdot 0 + 0 \cdot \sqrt{2}/2 = \sqrt{2}/2\)
  - Second element: \(1 \cdot 0 + 0 \cdot 1 + 0 \cdot 0 = 0\)
  - Third element: \(1 \cdot (-\sqrt{2}/2) + 0 \cdot 0 + 0 \cdot \sqrt{2}/2 = -\sqrt{2}/2\)

- **Second row:**
  - First element: \(0 \cdot \sqrt{2}/2 + (\sqrt{3}/2) \cdot 0 + (1/2) \cdot \sqrt{2}/2 = 0 + 0 + (1/2) \cdot \sqrt{2}/2 = \sqrt{2}/4\)
  - Second element: \(0 \cdot 0 + (\sqrt{3}/2) \cdot 1 + (1/2) \cdot 0 = \sqrt{3}/2\)
  - Third element: \(0 \cdot (-\sqrt{2}/2) + (\sqrt{3}/2) \cdot 0 + (1/2) \cdot \sqrt{2}/2 = 0 + 0 + (1/2) \cdot \sqrt{2}/2 = \sqrt{2}/4\)

- **Third row:**
  - First element: \(0 \cdot \sqrt{2}/2 + (-1/2) \cdot 0 + (\sqrt{3}/2) \cdot \sqrt{2}/2 = 0 + 0 + (\sqrt{3}/2) \cdot \sqrt{2}/2 = \sqrt{6}/4\)
  - Second element: \(0 \cdot 0 + (-1/2) \cdot 1 + (\sqrt{3}/2) \cdot 0 = -1/2\)
  - Third element: \(0 \cdot (-\sqrt{2}/2) + (-1/2) \cdot 0 + (\sqrt{3}/2) \cdot \sqrt{2}/2 = 0 + 0 + (\sqrt{3}/2) \cdot \sqrt{2}/2 = \sqrt{6}/4\)
```

Thus, the rotation matrix from T to R is:

```math
\[
^R\mathbf{R}_T = \begin{pmatrix}
\frac{\sqrt{2}}{2} & 0 & -\frac{\sqrt{2}}{2} \\
\frac{\sqrt{2}}{4} & \frac{\sqrt{3}}{2} & \frac{\sqrt{2}}{4} \\
\frac{\sqrt{6}}{4} & -\frac{1}{2} & \frac{\sqrt{6}}{4}
\end{pmatrix}
\]
```

This matrix transforms vectors from the tool frame T to the robot frame R.

```math
\boxed{ \begin{pmatrix} \frac{\sqrt{2}}{2} & 0 & -\frac{\sqrt{2}}{2} \\ \frac{\sqrt{2}}{4} & \frac{\sqrt{3}}{2} & \frac{\sqrt{2}}{4} \\ \frac{\sqrt{6}}{4} & -\frac{1}{2} & \frac{\sqrt{6}}{4} \end{pmatrix} }
```

## Grok 3

To find the 3×3 rotation matrix from tool frame T to robot frame R (i.e., ( R_T^R )), we need to compute the composition of the rotation matrices that describe the transformations between the frames. Let's break this down step by step.

### Step 1: Understand the transformations

1. **Frame G relative to Frame R**: Gripper frame G is rotated 30° about the X-axis relative to robot frame R. This means we need the rotation matrix ( R_G^R ), which represents a rotation of 30° about the X-axis.
1. **Frame T relative to Frame G**: Tool frame T is rotated 45° about the Y-axis relative to gripper frame G. This means we need the rotation matrix ( R_T^G ), which represents a rotation of 45° about the Y-axis.
1. **Frame T relative to Frame R**: The desired rotation matrix ( R_T^R ) is the composition of the two rotations: ( R_T^R = R_G^R \\cdot R_T^G ).

### Step 2: Define the individual rotation matrices

- **Rotation about X-axis by 30° (( R_G^R ))**:\
  A rotation by an angle ( \\theta ) about the X-axis is given by:
  \[
  R_X(\\theta) = \\begin{bmatrix}
  1 & 0 & 0 \\
  0 & \\cos\\theta & -\\sin\\theta \\
  0 & \\sin\\theta & \\cos\\theta
  \\end{bmatrix}
  \]
  For ( \\theta = 30^\\circ ), we have ( \\cos 30^\\circ = \\frac{\\sqrt{3}}{2} \\approx 0.866 ), and ( \\sin 30^\\circ = 0.5 ). Thus:
  \[
  R_G^R = \\begin{bmatrix}
  1 & 0 & 0 \\
  0 & 0.866 & -0.5 \\
  0 & 0.5 & 0.866
  \\end{bmatrix}
  \]

- **Rotation about Y-axis by 45° (( R_T^G ))**:\
  A rotation by an angle ( \\theta ) about the Y-axis is given by:
  \[
  R_Y(\\theta) = \\begin{bmatrix}
  \\cos\\theta & 0 & \\sin\\theta \\
  0 & 1 & 0 \\
  -\\sin\\theta & 0 & \\cos\\theta
  \\end{bmatrix}
  \]
  For ( \\theta = 45^\\circ ), we have ( \\cos 45^\\circ = \\sin 45^\\circ = \\frac{\\sqrt{2}}{2} \\approx 0.707 ). Thus:
  \[
  R_T^G = \\begin{bmatrix}
  0.707 & 0 & 0.707 \\
  0 & 1 & 0 \\
  -0.707 & 0 & 0.707
  \\end{bmatrix}
  \]

### Step 3: Compute the composite rotation matrix ( R_T^R )

Since ( R_T^R = R_G^R \\cdot R_T^G ), we multiply the two matrices:
\[
R_T^R = \\begin{bmatrix}
1 & 0 & 0 \\
0 & 0.866 & -0.5 \\
0 & 0.5 & 0.866
\\end{bmatrix}
\\cdot
\\begin{bmatrix}
0.707 & 0 & 0.707 \\
0 & 1 & 0 \\
-0.707 & 0 & 0.707
\\end{bmatrix}
\]

Let's compute this matrix multiplication element by element.

#### First row of ( R_T^R ):

- ( R_T^R[1,1] = 1 \\cdot 0.707 + 0 \\cdot 0 + 0 \\cdot (-0.707) = 0.707 )
- ( R_T^R[1,2] = 1 \\cdot 0 + 0 \\cdot 1 + 0 \\cdot 0 = 0 )
- ( R_T^R[1,3] = 1 \\cdot 0.707 + 0 \\cdot 0 + 0 \\cdot 0.707 = 0.707 )

#### Second row of ( R_T^R ):

- ( R_T^R[2,1] = 0 \\cdot 0.707 + 0.866 \\cdot 0 + (-0.5) \\cdot (-0.707) = 0.3535 )
- ( R_T^R[2,2] = 0 \\cdot 0 + 0.866 \\cdot 1 + (-0.5) \\cdot 0 = 0.866 )
- ( R_T^R[2,3] = 0 \\cdot 0.707 + 0.866 \\cdot 0 + (-0.5) \\cdot 0.707 = -0.3535 )

#### Third row of ( R_T^R ):

- ( R_T^R[3,1] = 0 \\cdot 0.707 + 0.5 \\cdot 0 + 0.866 \\cdot (-0.707) = -0.6122 )
- ( R_T^R[3,2] = 0 \\cdot 0 + 0.5 \\cdot 1 + 0.866 \\cdot 0 = 0.5 )
- ( R_T^R[3,3] = 0 \\cdot 0.707 + 0.5 \\cdot 0 + 0.866 \\cdot 0.707 = 0.6122 )

Thus, the rotation matrix ( R_T^R ) is:
\[
R_T^R = \\begin{bmatrix}
0.707 & 0 & 0.707 \\
0.3535 & 0.866 & -0.3535 \\
-0.6122 & 0.5 & 0.6122
\\end{bmatrix}
\]

### Step 4: Verify and present the final answer

To ensure accuracy, note that the values are approximate due to rounding of trigonometric functions. If higher precision is needed, the exact values (e.g., ( \\cos 30^\\circ = \\frac{\\sqrt{3}}{2} ), ( \\sin 45^\\circ = \\frac{\\sqrt{2}}{2} )) can be used.

The final 3×3 rotation matrix from frame T to frame R is:
\[
R_T^R = \\begin{bmatrix}
\\frac{\\sqrt{2}}{2} & 0 & \\frac{\\sqrt{2}}{2} \\
\\frac{\\sqrt{6}}{4} & \\frac{\\sqrt{3}}{2} & -\\frac{\\sqrt{6}}{4} \\
-\\frac{\\sqrt{6}}{4} & \\frac{1}{2} & \\frac{\\sqrt{6}}{4}
\\end{bmatrix}
\]
Or, with numerical approximations:
\[
R_T^R \\approx \\begin{bmatrix}
0.707 & 0 & 0.707 \\
0.354 & 0.866 & -0.354 \\
-0.612 & 0.5 & 0.612
\\end{bmatrix}
\]
