# Prompt #48: Orthographically project (7, −3, 5, 2) onto w = 0, then rotate the result 90° about the z-axis. State the final 3-D point.

## OpenAI o3  (18 secs)
Step 1 :  Orthographic projection onto the plane w = 0  
Dropping the w–coordinate simply gives the 3-D point  
P = (7, −3, 5).

Step 2 :  90° rotation about the z-axis  
For a counter-clockwise 90° rotation about the z-axis  

 x′ = x cos 90° − y sin 90° = 0·x − 1·y = −y  
 y′ = x sin 90° + y cos 90° = 1·x + 0·y = x  
 z′ = z  

Substituting x = 7, y = −3, z = 5:

 x′ = −(−3) = 3  
 y′ = 7  
 z′ = 5

Final 3-D point: (3, 7, 5).

## Claude 4 Sonnet  (12 secs)
I need to orthographically project the 4D point (7, -3, 5, 2) onto the hyperplane w = 0, then rotate the resulting 3D point 90° about the z-axis.

Step 1: Orthographic projection onto w = 0

When we project a 4D point (x, y, z, w) onto the hyperplane w = 0, we simply drop the w-coordinate, keeping the (x, y, z) components unchanged.

So projecting (7, -3, 5, 2) onto w = 0 gives us:
(7, -3, 5)

Step 2: Rotate 90° about the z-axis

A 90° rotation about the z-axis transforms coordinates according to:
- x' = -y
- y' = x  
- z' = z

This is because a 90° counterclockwise rotation about the z-axis has the rotation matrix:
```
[cos(90°)  -sin(90°)  0]   [0  -1  0]
[sin(90°)   cos(90°)  0] = [1   0  0]
[   0          0      1]   [0   0  1]
```

Applying this to our point (7, -3, 5):
- x' = -(-3) = 3
- y' = 7
- z' = 5

Therefore, the final 3D point is **(3, 7, 5)**.

## Gemini Pro  (62 secs)
Let the given 4-dimensional point be $P_4 = (x_4, y_4, z_4, w_4) = (7, -3, 5, 2)$.

Step 1: Orthographically project the point onto $w=0$.
Orthographic projection onto $w=0$ means that the $w$-coordinate of the point becomes 0, while the other coordinates remain unchanged.
So, the projected point in 4D space is $P'_{4D} = (7, -3, 5, 0)$.

To obtain a 3-D point from this 4D point in the $w=0$ subspace, we typically drop the $w$-coordinate.
So, the resulting 3-D point is $P_3 = (x, y, z) = (7, -3, 5)$.

Step 2: Rotate the result 90° about the z-axis.
The point to be rotated is $(x, y, z) = (7, -3, 5)$.
A rotation about the z-axis means that the z-coordinate remains unchanged.
The rotation transformation for the x and y coordinates by an angle $\theta$ counter-clockwise is:
$x' = x \cos \theta - y \sin \theta$
$y' = x \sin \theta + y \cos \theta$
$z' = z$

In this problem, the rotation angle is $\theta = 90°$.
We have $\cos 90° = 0$ and $\sin 90° = 1$.
So the transformation becomes:
$x' = x(0) - y(1) = -y$
$y' = x(1) + y(0) = x$
$z' = z$

Now, we apply this transformation to the point $(7, -3, 5)$:
$x = 7$
$y = -3$
$z = 5$

The new coordinates are:
$x' = -(-3) = 3$
$y' = 7$
$z' = 5$

The final 3-D point after the rotation is $(3, 7, 5)$.

This assumes standard conventions:
1.  The coordinates of the 4D point are given in the order $(x, y, z, w)$.
2.  The projection onto $w=0$ means the fourth component is set to zero.
3.  The resulting 3D point $(x,y,z)$ is formed by the first three components.
4.  Rotation by $90°$ implies counter-clockwise rotation, following the right-hand rule (if thumb points along positive z-axis, fingers curl in the direction of positive rotation).

The final answer is $\boxed{(3,7,5)}$.

## DeepSeek Reasoner  (68 secs)
The orthographic projection of the point \((7, -3, 5, 2)\) onto the hyperplane \(w = 0\) sets the \(w\)-coordinate to 0, resulting in the 3-D point \((7, -3, 5)\).

Next, rotate this point 90 degrees counterclockwise about the \(z\)-axis. The rotation about the \(z\)-axis by an angle \(\theta = 90^\circ\) uses the rotation matrix:
\[
\begin{bmatrix}
x' \\
y' \\
z'
\end{bmatrix}
=
\begin{bmatrix}
\cos 90^\circ & -\sin 90^\circ & 0 \\
\sin 90^\circ & \cos 90^\circ & 0 \\
0 & 0 & 1
\end{bmatrix}
\begin{bmatrix}
x \\
y \\
z
\end{bmatrix}
\]
Since \(\cos 90^\circ = 0\) and \(\sin 90^\circ = 1\), this simplifies to:
\[
x' = -y, \quad y' = x, \quad z' = z.
\]

Applying this to the point \((7, -3, 5)\):
- \(x' = -(-3) = 3\)
- \(y' = 7\)
- \(z' = 5\)

Thus, the rotated point is \((3, 7, 5)\).

The final 3-D point is \((3, 7, 5)\).

\boxed{(3,7,5)}

## Grok 3  (5 secs)
Let's solve this problem step by step. We are given a 4D point \((7, -3, 5, 2)\) and need to orthographically project it onto the hyperplane where \(w = 0\), then rotate the result 90° about the z-axis in 3D space, and finally state the resulting 3D point.

### Step 1: Orthographic Projection onto \(w = 0\)
Orthographic projection onto the hyperplane \(w = 0\) means we simply ignore the \(w\)-coordinate of the 4D point and take the first three coordinates as the 3D point. So, for the point \((7, -3, 5, 2)\), the projection onto \(w = 0\) (i.e., the 3D space) is:

\[
(7, -3, 5)
\]

This is because orthographic projection in this context drops the fourth coordinate.

### Step 2: Rotate the Result 90° About the z-Axis
Now we have the 3D point \((7, -3, 5)\), and we need to rotate it 90° counterclockwise about the z-axis. Rotation about the z-axis affects only the \(x\)- and \(y\)-coordinates, while the \(z\)-coordinate remains unchanged.

The transformation for a 90° counterclockwise rotation about the z-axis is given by the rotation matrix:

\[
R_z(90^\circ) = \begin{bmatrix}
\cos(90^\circ) & -\sin(90^\circ) & 0 \\
\sin(90^\circ) & \cos(90^\circ) & 0 \\
0 & 0 & 1
\end{bmatrix}
= \begin{bmatrix}
0 & -1 & 0 \\
1 & 0 & 0 \\
0 & 0 & 1
\end{bmatrix}
\]

Applying this rotation to the point \((7, -3, 5)\), we compute the new coordinates as follows:

- New \(x' = 0 \cdot 7 + (-1) \cdot (-3) + 0 \cdot 5 = 0 + 3 + 0 = 3\)
- New \(y' = 1 \cdot 7 + 0 \cdot (-3) + 0 \cdot 5 = 7 + 0 + 0 = 7\)
- New \(z' = 0 \cdot 7 + 0 \cdot (-3) + 1 \cdot 5 = 0 + 0 + 5 = 5\)

Thus, after rotation, the point becomes:

\[
(3, 7, 5)
\]

### Final Answer
The final 3D point after orthographic projection and rotation is:

\[
(3, 7, 5)
\]

